Pm4Lean/Models.lean
@@ -9,5 +9,3 @@ import Pm4Lean.Models.Language
 import Pm4Lean.Models.Petri
 import Pm4Lean.Models.POWL
 import Pm4Lean.Models.POWL2
--- import Pm4Lean.Models.ProcessTree
--- import Pm4Lean.Models.BPMN
