Pm4Lean/Models/BPMN.lean
@@ -1,1 +1,0 @@
-import Pm4Lean.Models.BPMN.Examples
