Pm4Lean/Models/ProcessTree.lean
@@ -1,2 +1,0 @@
-import Pm4Lean.Models.ProcessTree.Basic
-import Pm4Lean.Models.ProcessTree.Semantics
